Clean up instantiation of symbolic logic variables

src/MicroSail/Sep/Spec.v
@@ -98,14 +98,8 @@ Module Assertions
   (*   | asn_exist ς τ a => asn_exist ς τ (sub_assertion (sub_up1 ζ) a) *)
   (*   end. *)
 
-  Definition SymbolicLocalStore (Γ : Ctx (𝑿 * Ty)) (Σ : Ctx (𝑺 * Ty)) : Type :=
-    NamedEnv (Term Σ) Γ.
-  Bind Scope env_scope with SymbolicLocalStore.
   (* Definition SymbolicRegStore (Σ : Ctx (𝑺 * Ty))  : Type := forall σ, 𝑹𝑬𝑮 σ -> Term Σ σ. *)
 
-  Definition eval_symLocalStore {Γ Σ}
-    (δ : SymbolicLocalStore Γ Σ) (δΣ : NamedEnv Lit Σ) : LocalStore Γ :=
-    env_map (fun _ t => eval_term t δΣ) δ.
 
   Definition symbolic_eval_exp {Γ Σ} (δ : SymbolicLocalStore Γ Σ) :
     forall {σ} (e : Exp Γ σ), Term Σ σ :=
