src/MicroSail/Sep/Hoare.v
@@ -18,272 +18,287 @@ Module ProgramLogic
   Import CtxNotations.
   Import EnvNotations.
 
-  (* Some simple instance that make writing program logic rules more natural by
-   avoiding the need to mention the local variable store δ in the pre and post
-   conditions that don't affect it *)
-  Section WithΓ.
-    Context (Γ : Ctx (𝑿 * Ty)).
+  (* (* Some simple instance that make writing program logic rules more natural by *)
+  (*  avoiding the need to mention the local variable store δ in the pre and post *)
+  (*  conditions that don't affect it *) *)
+  (* Section WithΓ. *)
+  (*   Context (Γ : Ctx (𝑿 * Ty)). *)
 
-    Instance δ_ILogic (L : Type) (LL : ILogic L) : ILogic (LocalStore Γ -> L) :=
-      { lentails P Q := (forall δ, lentails (P δ ) (Q δ));
-        ltrue := (fun _ => ltrue);
-        lfalse := (fun _ => lfalse);
-        land P Q := (fun δ => (land (P δ) (Q δ)));
-        lor P Q := (fun δ => (lor (P δ) (Q δ)));
-        limpl P Q := (fun δ => (limpl (P δ) (Q δ)));
-        lprop P := fun _ => lprop P;
-        lex {T} (F : T -> LocalStore Γ -> L) := fun δ => lex (fun t => F t δ);
-        lall {T} (F : T -> LocalStore Γ -> L) := fun δ => lall (fun t => F t δ)
-      }.
+  (*   Instance δ_ILogic (L : Type) (LL : ILogic L) : ILogic (LocalStore Γ -> L) := *)
+  (*     { lentails P Q := (forall δ, lentails (P δ ) (Q δ)); *)
+  (*       ltrue := (fun _ => ltrue); *)
+  (*       lfalse := (fun _ => lfalse); *)
+  (*       land P Q := (fun δ => (land (P δ) (Q δ))); *)
+  (*       lor P Q := (fun δ => (lor (P δ) (Q δ))); *)
+  (*       limpl P Q := (fun δ => (limpl (P δ) (Q δ))); *)
+  (*       lprop P := fun _ => lprop P; *)
+  (*       lex {T} (F : T -> LocalStore Γ -> L) := fun δ => lex (fun t => F t δ); *)
+  (*       lall {T} (F : T -> LocalStore Γ -> L) := fun δ => lall (fun t => F t δ) *)
+  (*     }. *)
 
-    Program Instance δ_ILogicLaws (L : Type) (LL : ILogic L) (LLL : ILogicLaws L LL) :
-      ILogicLaws (LocalStore Γ -> L) (δ_ILogic L LL).
-    (* (* Solve the obligations with firstorder take a lot of time. *) *)
-    (* Solve Obligations with firstorder. *)
-    Admit Obligations.
+  (*   Program Instance δ_ILogicLaws (L : Type) (LL : ILogic L) (LLL : ILogicLaws L LL) : *)
+  (*     ILogicLaws (LocalStore Γ -> L) (δ_ILogic L LL). *)
+  (*   (* (* Solve the obligations with firstorder take a lot of time. *) *) *)
+  (*   (* Solve Obligations with firstorder. *) *)
+  (*   Admit Obligations. *)
 
-    Instance δ_ISepLogic (L : Type) (SL : ISepLogic L) : ISepLogic (LocalStore Γ -> L) :=
-      { emp := fun _ => emp;
-        sepcon P Q := fun δ => sepcon (P δ) (Q δ);
-        wand P Q := fun δ => wand (P δ) (Q δ)
-      }.
+  (*   Instance δ_ISepLogic (L : Type) (SL : ISepLogic L) : ISepLogic (LocalStore Γ -> L) := *)
+  (*     { emp := fun _ => emp; *)
+  (*       sepcon P Q := fun δ => sepcon (P δ) (Q δ); *)
+  (*       wand P Q := fun δ => wand (P δ) (Q δ) *)
+  (*     }. *)
 
-    Program Instance δ_ISepLogicLaws (L : Type) (LL : ISepLogic L) (LLL : ISepLogicLaws L) :
-      ISepLogicLaws (LocalStore Γ -> L).
-    Admit Obligations.
+  (*   Program Instance δ_ISepLogicLaws (L : Type) (LL : ISepLogic L) (LLL : ISepLogicLaws L) : *)
+  (*     ISepLogicLaws (LocalStore Γ -> L). *)
+  (*   Admit Obligations. *)
 
-    Program Instance δ_IHeaplet (L : Type) (SL : IHeaplet L) :
-      IHeaplet (LocalStore Γ -> L) :=
-      { pred p ts := fun δ => pred p ts;
-        ptsreg σ r v := fun δ => ptsreg r v
-      }.
+  (*   Program Instance δ_IHeaplet (L : Type) (SL : IHeaplet L) : *)
+  (*     IHeaplet (LocalStore Γ -> L) := *)
+  (*     { pred p ts := fun δ => pred p ts; *)
+  (*       ptsreg σ r v := fun δ => ptsreg r v *)
+  (*     }. *)
 
-  End WithΓ.
+  (* End WithΓ. *)
+
+  (* Existing Instance δ_IHeaplet. *)
+
 
   Open Scope logic.
 
-  Reserved Notation "δ ⊢ ⦃ P ⦄ s ⦃ Q ⦄" (at level 75, no associativity).
+  Section Triples.
 
-  Existing Instance δ_IHeaplet.
+    Context {L : Type}.
+    Context {LL : IHeaplet L}.
 
-  (* Hoare triples for SepContract *)
+    (* Hoare triples for SepContract *)
 
-  Inductive CTriple {L : Type} {Logic : IHeaplet L} (Δ : Ctx (𝑿 * Ty)) (δΔ : LocalStore Δ)
-            {σ : Ty} :
-    forall (pre : L) (post : Lit σ -> L) (c : SepContract Δ σ), Prop :=
-  (* | rule_sep_contract_unit *)
-  (*     (Σ  : Ctx (𝑺 * Ty)) (θΔ : SymbolicLocalStore Δ Σ) (δΣ : NamedEnv Lit Σ) *)
-  (*     (req : Assertion Σ) (ens : Assertion Σ) : *)
-  (*     δΔ = env_map (fun _ t => eval_term t δΣ) θΔ -> *)
-  (*     CTriple (τ:=ty_unit) Δ δΔ *)
-  (*       (interpret δΣ req) *)
-  (*       (fun _ => interpret δΣ ens) *)
-  (*       (sep_contract_unit θΔ req ens) *)
-  | rule_sep_contract_result_pure
-      (Σ  : Ctx (𝑺 * Ty)) (θΔ : SymbolicLocalStore Δ Σ) (δΣ : NamedEnv Lit Σ)
-      (req : Assertion Σ) (ens : Assertion Σ) (result : Term Σ σ) :
-      δΔ = env_map (fun _ t => eval_term t δΣ) θΔ ->
-      CTriple Δ δΔ
-        (interpret δΣ req)
-        (fun v => interpret δΣ ens ∧ !!(v = eval_term result δΣ))
-        (sep_contract_result_pure θΔ result req ens)
-  | rule_sep_contract_result
-      (result : 𝑺)
-      (Σ  : Ctx (𝑺 * Ty)) (θΔ : SymbolicLocalStore Δ Σ) (δΣ : NamedEnv Lit Σ)
-      (req : Assertion Σ) (ens : Assertion (Σ ▻ (result , σ))) :
-      δΔ = env_map (fun _ t => eval_term t δΣ) θΔ ->
-      CTriple
-        Δ δΔ
-        (interpret δΣ req)
-        (fun v => interpret (env_snoc δΣ (result , σ) v) ens)
-        (@sep_contract_result _ _ _ θΔ result req ens).
-  (* | rule_sep_contract_none {σ} : *)
-  (*     Pi f *)
-  (*     CTriple Γ (fun _ => ⊤) (fun _ _ => ⊤) (@sep_contract_none Γ σ). *)
+    Inductive CTriple (Δ : Ctx (𝑿 * Ty)) (δΔ : LocalStore Δ) {σ : Ty} :
+      forall (pre : L) (post : Lit σ -> L) (c : SepContract Δ σ), Prop :=
+    (* | rule_sep_contract_unit *)
+    (*     (Σ  : Ctx (𝑺 * Ty)) (θΔ : SymbolicLocalStore Δ Σ) (ι : SymInstance Σ) *)
+    (*     (req : Assertion Σ) (ens : Assertion Σ) : *)
+    (*     δΔ = inst_localstore ι θΔ -> *)
+    (*     CTriple (τ:=ty_unit) Δ δΔ *)
+    (*       (inst_assertion ι req) *)
+    (*       (fun _ => inst_assertion ι ens) *)
+    (*       (sep_contract_unit θΔ req ens) *)
+    | rule_sep_contract_result_pure
+        (Σ  : Ctx (𝑺 * Ty)) (θΔ : SymbolicLocalStore Δ Σ) (ι : SymInstance Σ)
+        (req : Assertion Σ) (ens : Assertion Σ) (result : Term Σ σ) :
+        δΔ = inst_localstore ι θΔ ->
+        CTriple Δ δΔ
+          (inst_assertion ι req)
+          (fun v => inst_assertion ι ens ∧ !!(v = inst_term ι result))
+          (sep_contract_result_pure θΔ result req ens)
+    | rule_sep_contract_result
+        (result : 𝑺)
+        (Σ  : Ctx (𝑺 * Ty)) (θΔ : SymbolicLocalStore Δ Σ) (ι : SymInstance Σ)
+        (req : Assertion Σ) (ens : Assertion (Σ ▻ (result , σ))) :
+        δΔ = inst_localstore ι θΔ ->
+        CTriple
+          Δ δΔ
+          (inst_assertion ι req)
+          (fun v => inst_assertion (env_snoc ι (result , σ) v) ens)
+          (@sep_contract_result _ _ _ θΔ result req ens).
+    (* | rule_sep_contract_none {σ} : *)
+    (*     Pi f *)
+    (*     CTriple Γ (fun _ => ⊤) (fun _ _ => ⊤) (@sep_contract_none Γ σ). *)
 
 
-  Inductive Triple {L : Type} {Logic : IHeaplet L} (Γ : Ctx (𝑿 * Ty)) (δ : LocalStore Γ) :
-    forall {τ : Ty}
-      (pre : L) (s : Stm Γ τ)
-      (post :  Lit τ -> LocalStore Γ -> L), Prop :=
-  | rule_consequence {σ : Ty}
-      {P P' : L} {Q Q' : Lit σ -> LocalStore Γ -> L} {s : Stm Γ σ} :
-      (P ⊢ P') -> (forall v δ', Q' v δ' ⊢ Q v δ') -> δ ⊢ ⦃ P' ⦄ s ⦃ Q' ⦄ -> δ ⊢ ⦃ P ⦄ s ⦃ Q ⦄
-  | rule_frame {σ : Ty}
-      (R P : L) (Q : Lit σ -> LocalStore Γ -> L) (s : Stm Γ σ) :
-      δ ⊢ ⦃ P ⦄ s ⦃ Q ⦄ -> δ ⊢ ⦃ R ✱ P ⦄ s ⦃ fun v δ' => R ✱ Q v δ' ⦄
-  | rule_pull
-      {σ : Ty} (s : Stm Γ σ)
-      (P : L) (Q : Prop) (R : Lit σ -> LocalStore Γ -> L) :
-      (Q -> δ ⊢ ⦃ P ⦄ s ⦃ R ⦄) ->
-      δ ⊢ ⦃ P ∧ !!Q ⦄ s ⦃ R ⦄
-  | rule_stm_lit
-      {τ : Ty} {l : Lit τ}
-      {P : L} {Q : Lit τ -> LocalStore Γ -> L} :
-      P ⊢ Q l δ ->
-      δ ⊢ ⦃ P ⦄ stm_lit τ l ⦃ Q ⦄
-  | rule_stm_exp
-      {τ : Ty} {e : Exp Γ τ}
-      {P : L} {Q : Lit τ -> LocalStore Γ -> L} :
-      P ⊢ Q (eval e δ) δ ->
-      δ ⊢ ⦃ P ⦄ stm_exp e ⦃ Q ⦄
-  | rule_stm_let
-      (x : 𝑿) (σ τ : Ty) (s : Stm Γ σ) (k : Stm (ctx_snoc Γ (x , σ)) τ)
-      (P : L) (Q : Lit σ -> LocalStore Γ -> L)
-      (R : Lit τ -> LocalStore Γ -> L) :
-      δ         ⊢ ⦃ P ⦄ s ⦃ Q ⦄ ->
-      (forall (v : Lit σ) (δ' : LocalStore Γ),
-          env_snoc δ' (x,σ) v ⊢ ⦃ Q v δ' ⦄ k ⦃ fun v δ'' => R v (env_tail δ'') ⦄ ) ->
-      δ         ⊢ ⦃ P ⦄ let: x := s in k ⦃ R ⦄
-  | rule_stm_let_forwards
-      (x : 𝑿) (σ τ : Ty) (s : Stm Γ σ) (k : Stm (ctx_snoc Γ (x , σ)) τ)
-      (P : L) (Q : Lit σ -> LocalStore Γ -> L)
-      (R : Lit τ -> LocalStore (Γ ▻ (x,σ)) -> L) :
-      δ         ⊢ ⦃ P ⦄ s ⦃ Q ⦄ ->
-      (forall (v : Lit σ) (δ' : LocalStore Γ),
-          env_snoc δ' (x,σ) v ⊢ ⦃ Q v δ' ⦄ k ⦃ R ⦄ ) ->
-      δ         ⊢ ⦃ P ⦄ let: x := s in k ⦃ fun v δ' => ∃ v__let, R v (env_snoc δ' (x,σ) v__let)⦄
-  | rule_stm_block
-      (Δ : Ctx (𝑿 * Ty)) (δΔ : LocalStore Δ)
-      (τ : Ty) (k : Stm (ctx_cat Γ Δ) τ)
-      (P : L) (R : Lit τ -> LocalStore Γ -> L) :
-      (δ ►► δΔ ⊢ ⦃ P ⦄ k ⦃ fun v δ'' => R v (env_drop Δ δ'') ⦄) ->
-      δ         ⊢ ⦃ P ⦄ stm_block δΔ k ⦃ R ⦄
-  | rule_stm_if
-      (τ : Ty) (e : Exp Γ ty_bool) (s1 s2 : Stm Γ τ)
-      (P : L) (Q : Lit τ -> LocalStore Γ -> L) :
-      δ ⊢ ⦃ P ∧ !!(eval e δ = true) ⦄ s1 ⦃ Q ⦄ ->
-      δ ⊢ ⦃ P ∧ !!(eval e δ = false) ⦄ s2 ⦃ Q ⦄ ->
-      δ ⊢ ⦃ P ⦄ stm_if e s1 s2 ⦃ Q ⦄
-  | rule_stm_if_backwards
-      (τ : Ty) (e : Exp Γ ty_bool) (s1 s2 : Stm Γ τ)
-      (P1 P2 : L) (Q : Lit τ -> LocalStore Γ -> L) :
-      δ ⊢ ⦃ P1 ⦄ s1 ⦃ Q ⦄ -> δ ⊢ ⦃ P2 ⦄ s2 ⦃ Q ⦄ ->
-      δ ⊢ ⦃ (!!(eval e δ = true)  --> P1) ∧
-            (!!(eval e δ = false) --> P2)
-          ⦄ stm_if e s1 s2 ⦃ Q ⦄
-  | rule_stm_seq
-      (τ : Ty) (s1 : Stm Γ τ) (σ : Ty) (s2 : Stm Γ σ)
-      (P : L) (Q : LocalStore Γ -> L) (R : Lit σ -> LocalStore Γ -> L) :
-      δ ⊢ ⦃ P ⦄ s1 ⦃ fun _ => Q ⦄ ->
-      (forall δ', δ' ⊢ ⦃ Q δ' ⦄ s2 ⦃ R ⦄) ->
-      δ ⊢ ⦃ P ⦄ s1 ;; s2 ⦃ R ⦄
-  | rule_stm_assert (e1 : Exp Γ ty_bool) (e2 : Exp Γ ty_string)
-                    (P : L) :
-      δ ⊢ ⦃ P ⦄ stm_assert e1 e2 ⦃ fun v δ' => P ∧ !!(δ = δ' /\ eval e1 δ' = v /\ v = true) ⦄
-  | rule_stm_fail (τ : Ty) (s : Lit ty_string) :
-      forall (Q : Lit τ -> LocalStore Γ -> L),
-        δ ⊢ ⦃ ⊤ ⦄ stm_fail τ s ⦃ Q ⦄
-  | rule_stm_match_list
-      {σ τ : Ty} (e : Exp Γ (ty_list σ)) (alt_nil : Stm Γ τ)
-      (xh xt : 𝑿) (alt_cons : Stm (ctx_snoc (ctx_snoc Γ (xh , σ)) (xt , ty_list σ)) τ)
-      (Pnil : L) (Pcons : L) (Q : Lit τ -> LocalStore Γ -> L) :
-      δ ⊢ ⦃ Pnil ⦄ alt_nil ⦃ fun v' δ' => Q v' δ' ⦄ ->
-      (forall v vs, env_snoc (env_snoc δ (xh,σ) v) (xt,ty_list σ) vs ⊢
-                      ⦃ Pcons ⦄ alt_cons ⦃ fun v' δ' => Q v' (env_tail (env_tail δ')) ⦄) ->
-      δ ⊢ ⦃ (!!(eval e δ = nil) --> Pnil)
-          ∧ (∀ v vs, !!(eval e δ = cons v vs) --> Pcons)
-          ⦄ stm_match_list e alt_nil xh xt alt_cons ⦃ Q ⦄
-  | rule_stm_match_sum (σinl σinr τ : Ty) (e : Exp Γ (ty_sum σinl σinr))
-                       (xinl : 𝑿) (alt_inl : Stm (ctx_snoc Γ (xinl , σinl)) τ)
-                       (xinr : 𝑿) (alt_inr : Stm (ctx_snoc Γ (xinr , σinr)) τ)
-                       (Pinl : L)
-                       (Pinr : L)
-                       (Q : Lit τ -> LocalStore Γ -> L) :
-      (forall v, env_snoc δ (xinl,σinl) v ⊢ ⦃ Pinl ⦄ alt_inl ⦃ fun v' δ' => Q v' (env_tail δ') ⦄) ->
-      (forall v, env_snoc δ (xinr,σinr) v ⊢ ⦃ Pinr ⦄ alt_inr ⦃ fun v' δ' => Q v' (env_tail δ') ⦄) ->
-      δ ⊢ ⦃ (∀ x, !!(eval e δ = inl x) --> Pinl)
-          ∧ (∀ x, !!(eval e δ = inr x) --> Pinr)
-          ⦄ stm_match_sum e xinl alt_inl xinr alt_inr ⦃ Q ⦄
-  | rule_stm_match_pair
-      {σ1 σ2 τ : Ty} (e : Exp Γ (ty_prod σ1 σ2))
-      (xl xr : 𝑿) (rhs : Stm (ctx_snoc (ctx_snoc Γ (xl , σ1)) (xr , σ2)) τ)
-      (P : L) (Q : Lit τ -> LocalStore Γ -> L) :
-      (forall vl vr,
-          env_snoc (env_snoc δ (xl, σ1) vl) (xr, σ2) vr ⊢
-            ⦃ P ⦄ rhs ⦃ fun v δ' => Q v (env_tail (env_tail δ')) ⦄) ->
-      δ ⊢ ⦃ P ⦄ stm_match_pair e xl xr rhs ⦃ Q ⦄
-  | rule_stm_match_enum
-      {E : 𝑬} (e : Exp Γ (ty_enum E)) {τ : Ty}
-      (alts : forall (K : 𝑬𝑲 E), Stm Γ τ)
-      (P : L) (Q : Lit τ -> LocalStore Γ -> L) :
-      (forall K, δ ⊢ ⦃ P ⦄ alts K ⦃ Q ⦄) ->
-      δ ⊢ ⦃ P ⦄ stm_match_enum E e alts ⦃ Q ⦄
-  | rule_stm_match_tuple
-      {σs : Ctx Ty} {Δ : Ctx (𝑿 * Ty)} (e : Exp Γ (ty_tuple σs))
-      (p : TuplePat σs Δ) {τ : Ty} (rhs : Stm (ctx_cat Γ Δ) τ)
-      (P : L) (Q : Lit τ -> LocalStore Γ -> L) :
-      (forall (δΔ : LocalStore Δ),
-          env_cat δ δΔ ⊢ ⦃ P ⦄ rhs ⦃ fun v δ' => Q v (env_drop Δ δ') ⦄) ->
-      δ ⊢ ⦃ P ⦄ stm_match_tuple e p rhs ⦃ Q ⦄
-  | rule_stm_match_union
-      {U : 𝑼} (e : Exp Γ (ty_union U)) {σ τ : Ty}
-      (alt__Δ : forall (K : 𝑼𝑲 U), Ctx (𝑿 * Ty))
-      (alt__p : forall (K : 𝑼𝑲 U), Pattern (alt__Δ K) (𝑼𝑲_Ty K))
-      (alt__r : forall (K : 𝑼𝑲 U), Stm (ctx_cat Γ (alt__Δ K)) τ)
-      (P : forall (K : 𝑼𝑲 U), L) (Q : Lit τ -> LocalStore Γ -> L) :
-      (forall (K : 𝑼𝑲 U) (δΔ : LocalStore (alt__Δ K)),
-          env_cat δ δΔ ⊢ ⦃ P K ⦄ alt__r K ⦃ fun v δ' => Q v (env_drop (alt__Δ K) δ') ⦄) ->
-      δ ⊢
-        ⦃ ∀ (K : 𝑼𝑲 U) (v : Lit (𝑼𝑲_Ty K)), !!(eval e δ = 𝑼_fold (existT K v)) --> P K ⦄
-        stm_match_union U e (fun K => @alt Γ (𝑼𝑲_Ty K) τ (alt__Δ K) (alt__p K) (alt__r K))
-        ⦃ Q ⦄
-  | rule_stm_match_record
-      {R : 𝑹} {Δ : Ctx (𝑿 * Ty)} (e : Exp Γ (ty_record R))
-      (p : RecordPat (𝑹𝑭_Ty R) Δ) {τ : Ty} (rhs : Stm (ctx_cat Γ Δ) τ)
-      (P : L) (Q : Lit τ -> LocalStore Γ -> L) :
-      (forall (δΔ : LocalStore Δ),
-          env_cat δ δΔ ⊢ ⦃ P ⦄ rhs ⦃ fun v δ' => Q v (env_drop Δ δ') ⦄) ->
-      δ ⊢ ⦃ P ⦄ stm_match_record R e p rhs ⦃ Q ⦄
-  | rule_stm_read_register {σ : Ty} (r : 𝑹𝑬𝑮 σ) (v : Lit σ) :
-      δ ⊢ ⦃ r ↦ v ⦄ stm_read_register r ⦃ fun v' δ' => !!(δ' = δ) ∧ !!(v' = v) ∧ r ↦ v ⦄
-  (* | rule_stm_read_register_backwards {σ : Ty} (r : 𝑹𝑬𝑮 σ) *)
-  (*                                    (Q : Lit σ -> LocalStore Γ -> L) *)
-  (*                                    (v : Lit σ) : *)
-  (*     δ ⊢ ⦃ r ↦ v ✱ (r ↦ v -✱ Q v δ) ⦄ stm_read_register r ⦃ Q ⦄ *)
-  | rule_stm_write_register {σ : Ty} (r : 𝑹𝑬𝑮 σ) (w : Exp Γ σ)
-                            (Q : Lit σ -> LocalStore Γ -> L)
-                            (v : Lit σ) :
-      δ ⊢ ⦃ r ↦ v ⦄ stm_write_register r w ⦃ fun v' δ' => !!(δ' = δ) ∧ !!(v' = eval w δ)
-                                                       ∧ r ↦ v' ⦄
-  (* | rule_stm_write_register_backwards {σ : Ty} (r : 𝑹𝑬𝑮 σ) (w : Exp Γ σ) *)
-  (*                                     (Q : Lit σ -> LocalStore Γ -> L) *)
-  (*                                     (v : Lit σ) : *)
-  (*     δ ⊢ ⦃ r ↦ v ✱ (r ↦ eval w δ -✱ Q (eval w δ) δ) ⦄ stm_write_register r w ⦃ Q ⦄ *)
-  | rule_stm_assign_backwards
-      (x : 𝑿) (σ : Ty) (xIn : (x,σ) ∈ Γ) (s : Stm Γ σ)
-      (P : L) (R : Lit σ -> LocalStore Γ -> L) :
-      δ ⊢ ⦃ P ⦄ s ⦃ fun v δ' => R v (δ' ⟪ x ↦ v ⟫)%env ⦄ ->
-      δ ⊢ ⦃ P ⦄ stm_assign x s ⦃ R ⦄
-  | rule_stm_assign_forwards
-      (x : 𝑿) (σ : Ty) (xIn : (x,σ) ∈ Γ) (s : Stm Γ σ)
-      (P : L) (R : Lit σ -> LocalStore Γ -> L) :
-      δ ⊢ ⦃ P ⦄ s ⦃ R ⦄ ->
-      δ ⊢ ⦃ P ⦄ stm_assign x s ⦃ fun v__new δ' => ∃ v__old, R v__new (δ' ⟪ x ↦ v__old ⟫)%env ⦄
-  | rule_stm_call_forwards
-      {Δ σ} (f : 𝑭 Δ σ) (es : NamedEnv (Exp Γ) Δ)
-      (P : L)
-      (Q : Lit σ -> L) :
-      CTriple Δ (evals es δ) P Q (CEnv f) ->
-      δ ⊢ ⦃ P ⦄ stm_call f es ⦃ fun v δ' => Q v ∧ !!(δ = δ') ⦄
-  (* | rule_stm_call_backwards *)
-  (*     {Δ σ} (f : 𝑭 Δ σ) (es : NamedEnv (Exp Γ) Δ) *)
-  (*     (P : L) (Q : Lit σ -> LocalStore Γ -> L) : *)
-  (*     CTriple Δ (evals es δ) P (fun v => Q v δ) (CEnv f) -> *)
-  (*     δ ⊢ ⦃ P ⦄ stm_call f es ⦃ Q ⦄ *)
-  | rule_stm_call_frame
-      (Δ : Ctx (𝑿 * Ty)) (δΔ : LocalStore Δ) (τ : Ty) (s : Stm Δ τ)
-      (P : L) (Q : Lit τ -> LocalStore Γ -> L) :
-      δΔ ⊢ ⦃ P ⦄ s ⦃ fun v _ => Q v δ ⦄ ->
-      δ ⊢ ⦃ P ⦄ stm_call_frame Δ δΔ τ s ⦃ Q ⦄
-  | rule_stm_bind
-      {σ τ : Ty} (s : Stm Γ σ) (k : Lit σ -> Stm Γ τ)
-      (P : L) (Q : Lit σ -> LocalStore Γ -> L)
-      (R : Lit τ -> LocalStore Γ -> L) :
-      δ ⊢ ⦃ P ⦄ s ⦃ Q ⦄ ->
-      (forall (v__σ : Lit σ) (δ' : LocalStore Γ),
-          δ' ⊢ ⦃ Q v__σ δ' ⦄ k v__σ ⦃ R ⦄) ->
-      δ ⊢ ⦃ P ⦄ stm_bind s k ⦃ R ⦄
-  where "δ ⊢ ⦃ P ⦄ s ⦃ Q ⦄" := (Triple _ δ P s Q).
+    Inductive Triple {Γ : Ctx (𝑿 * Ty)} (δ : LocalStore Γ) :
+      forall {τ : Ty}
+        (pre : L) (s : Stm Γ τ)
+        (post :  Lit τ -> LocalStore Γ -> L), Prop :=
+    | rule_consequence {σ : Ty}
+        {P P' : L} {Q Q' : Lit σ -> LocalStore Γ -> L} {s : Stm Γ σ} :
+        (P ⊢ P') -> (forall v δ', Q' v δ' ⊢ Q v δ') -> δ ⊢ ⦃ P' ⦄ s ⦃ Q' ⦄ -> δ ⊢ ⦃ P ⦄ s ⦃ Q ⦄
+    | rule_frame {σ : Ty}
+        (R P : L) (Q : Lit σ -> LocalStore Γ -> L) (s : Stm Γ σ) :
+        δ ⊢ ⦃ P ⦄ s ⦃ Q ⦄ -> δ ⊢ ⦃ R ✱ P ⦄ s ⦃ fun v δ' => R ✱ Q v δ' ⦄
+    | rule_pull
+        {σ : Ty} (s : Stm Γ σ)
+        (P : L) (Q : Prop) (R : Lit σ -> LocalStore Γ -> L) :
+        (Q -> δ ⊢ ⦃ P ⦄ s ⦃ R ⦄) ->
+        δ ⊢ ⦃ P ∧ !!Q ⦄ s ⦃ R ⦄
+    | rule_stm_lit
+        {τ : Ty} {l : Lit τ}
+        {P : L} {Q : Lit τ -> LocalStore Γ -> L} :
+        P ⊢ Q l δ ->
+        δ ⊢ ⦃ P ⦄ stm_lit τ l ⦃ Q ⦄
+    | rule_stm_exp
+        {τ : Ty} {e : Exp Γ τ}
+        {P : L} {Q : Lit τ -> LocalStore Γ -> L} :
+        P ⊢ Q (eval e δ) δ ->
+        δ ⊢ ⦃ P ⦄ stm_exp e ⦃ Q ⦄
+    | rule_stm_let
+        (x : 𝑿) (σ τ : Ty) (s : Stm Γ σ) (k : Stm (ctx_snoc Γ (x , σ)) τ)
+        (P : L) (Q : Lit σ -> LocalStore Γ -> L)
+        (R : Lit τ -> LocalStore Γ -> L) :
+        δ         ⊢ ⦃ P ⦄ s ⦃ Q ⦄ ->
+        (forall (v : Lit σ) (δ' : LocalStore Γ),
+            env_snoc δ' (x,σ) v ⊢ ⦃ Q v δ' ⦄ k ⦃ fun v δ'' => R v (env_tail δ'') ⦄ ) ->
+        δ         ⊢ ⦃ P ⦄ let: x := s in k ⦃ R ⦄
+    | rule_stm_let_forwards
+        (x : 𝑿) (σ τ : Ty) (s : Stm Γ σ) (k : Stm (ctx_snoc Γ (x , σ)) τ)
+        (P : L) (Q : Lit σ -> LocalStore Γ -> L)
+        (R : Lit τ -> LocalStore (Γ ▻ (x,σ)) -> L) :
+        δ         ⊢ ⦃ P ⦄ s ⦃ Q ⦄ ->
+        (forall (v : Lit σ) (δ' : LocalStore Γ),
+            env_snoc δ' (x,σ) v ⊢ ⦃ Q v δ' ⦄ k ⦃ R ⦄ ) ->
+        δ         ⊢ ⦃ P ⦄ let: x := s in k ⦃ fun v δ' => ∃ v__let, R v (env_snoc δ' (x,σ) v__let)⦄
+    | rule_stm_block
+        (Δ : Ctx (𝑿 * Ty)) (δΔ : LocalStore Δ)
+        (τ : Ty) (k : Stm (ctx_cat Γ Δ) τ)
+        (P : L) (R : Lit τ -> LocalStore Γ -> L) :
+        (δ ►► δΔ ⊢ ⦃ P ⦄ k ⦃ fun v δ'' => R v (env_drop Δ δ'') ⦄) ->
+        δ         ⊢ ⦃ P ⦄ stm_block δΔ k ⦃ R ⦄
+    | rule_stm_if
+        (τ : Ty) (e : Exp Γ ty_bool) (s1 s2 : Stm Γ τ)
+        (P : L) (Q : Lit τ -> LocalStore Γ -> L) :
+        δ ⊢ ⦃ P ∧ !!(eval e δ = true) ⦄ s1 ⦃ Q ⦄ ->
+        δ ⊢ ⦃ P ∧ !!(eval e δ = false) ⦄ s2 ⦃ Q ⦄ ->
+        δ ⊢ ⦃ P ⦄ stm_if e s1 s2 ⦃ Q ⦄
+    | rule_stm_if_backwards
+        (τ : Ty) (e : Exp Γ ty_bool) (s1 s2 : Stm Γ τ)
+        (P1 P2 : L) (Q : Lit τ -> LocalStore Γ -> L) :
+        δ ⊢ ⦃ P1 ⦄ s1 ⦃ Q ⦄ -> δ ⊢ ⦃ P2 ⦄ s2 ⦃ Q ⦄ ->
+        δ ⊢ ⦃ (!!(eval e δ = true)  --> P1) ∧
+              (!!(eval e δ = false) --> P2)
+            ⦄ stm_if e s1 s2 ⦃ Q ⦄
+    | rule_stm_seq
+        (τ : Ty) (s1 : Stm Γ τ) (σ : Ty) (s2 : Stm Γ σ)
+        (P : L) (Q : LocalStore Γ -> L) (R : Lit σ -> LocalStore Γ -> L) :
+        δ ⊢ ⦃ P ⦄ s1 ⦃ fun _ => Q ⦄ ->
+        (forall δ', δ' ⊢ ⦃ Q δ' ⦄ s2 ⦃ R ⦄) ->
+        δ ⊢ ⦃ P ⦄ s1 ;; s2 ⦃ R ⦄
+    | rule_stm_assert (e1 : Exp Γ ty_bool) (e2 : Exp Γ ty_string)
+                      (P : L) :
+        δ ⊢ ⦃ P ⦄ stm_assert e1 e2 ⦃ fun v δ' => !!(δ = δ' /\ eval e1 δ' = v /\ v = true) ∧ P ⦄
+    | rule_stm_fail (τ : Ty) (s : Lit ty_string) :
+        forall (Q : Lit τ -> LocalStore Γ -> L),
+          δ ⊢ ⦃ ⊤ ⦄ stm_fail τ s ⦃ Q ⦄
+    | rule_stm_match_list
+        {σ τ : Ty} (e : Exp Γ (ty_list σ)) (alt_nil : Stm Γ τ)
+        (xh xt : 𝑿) (alt_cons : Stm (ctx_snoc (ctx_snoc Γ (xh , σ)) (xt , ty_list σ)) τ)
+        (Pnil : L) (Pcons : L) (Q : Lit τ -> LocalStore Γ -> L) :
+        δ ⊢ ⦃ Pnil ⦄ alt_nil ⦃ fun v' δ' => Q v' δ' ⦄ ->
+        (forall v vs, env_snoc (env_snoc δ (xh,σ) v) (xt,ty_list σ) vs ⊢
+                        ⦃ Pcons ⦄ alt_cons ⦃ fun v' δ' => Q v' (env_tail (env_tail δ')) ⦄) ->
+        δ ⊢ ⦃ (!!(eval e δ = nil) --> Pnil)
+            ∧ (∀ v vs, !!(eval e δ = cons v vs) --> Pcons)
+            ⦄ stm_match_list e alt_nil xh xt alt_cons ⦃ Q ⦄
+    | rule_stm_match_sum (σinl σinr τ : Ty) (e : Exp Γ (ty_sum σinl σinr))
+                         (xinl : 𝑿) (alt_inl : Stm (ctx_snoc Γ (xinl , σinl)) τ)
+                         (xinr : 𝑿) (alt_inr : Stm (ctx_snoc Γ (xinr , σinr)) τ)
+                         (Pinl : L)
+                         (Pinr : L)
+                         (Q : Lit τ -> LocalStore Γ -> L) :
+        (forall v, env_snoc δ (xinl,σinl) v ⊢ ⦃ Pinl ⦄ alt_inl ⦃ fun v' δ' => Q v' (env_tail δ') ⦄) ->
+        (forall v, env_snoc δ (xinr,σinr) v ⊢ ⦃ Pinr ⦄ alt_inr ⦃ fun v' δ' => Q v' (env_tail δ') ⦄) ->
+        δ ⊢ ⦃ (∀ x, !!(eval e δ = inl x) --> Pinl)
+            ∧ (∀ x, !!(eval e δ = inr x) --> Pinr)
+            ⦄ stm_match_sum e xinl alt_inl xinr alt_inr ⦃ Q ⦄
+    | rule_stm_match_pair
+        {σ1 σ2 τ : Ty} (e : Exp Γ (ty_prod σ1 σ2))
+        (xl xr : 𝑿) (rhs : Stm (ctx_snoc (ctx_snoc Γ (xl , σ1)) (xr , σ2)) τ)
+        (P : L) (Q : Lit τ -> LocalStore Γ -> L) :
+        (forall vl vr,
+            env_snoc (env_snoc δ (xl, σ1) vl) (xr, σ2) vr ⊢
+              ⦃ P ⦄ rhs ⦃ fun v δ' => Q v (env_tail (env_tail δ')) ⦄) ->
+        δ ⊢ ⦃ P ⦄ stm_match_pair e xl xr rhs ⦃ Q ⦄
+    | rule_stm_match_enum
+        {E : 𝑬} (e : Exp Γ (ty_enum E)) {τ : Ty}
+        (alts : forall (K : 𝑬𝑲 E), Stm Γ τ)
+        (P : L) (Q : Lit τ -> LocalStore Γ -> L) :
+        (forall K, δ ⊢ ⦃ P ⦄ alts K ⦃ Q ⦄) ->
+        δ ⊢ ⦃ P ⦄ stm_match_enum E e alts ⦃ Q ⦄
+    | rule_stm_match_tuple
+        {σs : Ctx Ty} {Δ : Ctx (𝑿 * Ty)} (e : Exp Γ (ty_tuple σs))
+        (p : TuplePat σs Δ) {τ : Ty} (rhs : Stm (ctx_cat Γ Δ) τ)
+        (P : L) (Q : Lit τ -> LocalStore Γ -> L) :
+        (forall (δΔ : LocalStore Δ),
+            env_cat δ δΔ ⊢ ⦃ P ⦄ rhs ⦃ fun v δ' => Q v (env_drop Δ δ') ⦄) ->
+        δ ⊢ ⦃ P ⦄ stm_match_tuple e p rhs ⦃ Q ⦄
+    | rule_stm_match_union
+        {U : 𝑼} (e : Exp Γ (ty_union U)) {σ τ : Ty}
+        (alt__Δ : forall (K : 𝑼𝑲 U), Ctx (𝑿 * Ty))
+        (alt__p : forall (K : 𝑼𝑲 U), Pattern (alt__Δ K) (𝑼𝑲_Ty K))
+        (alt__r : forall (K : 𝑼𝑲 U), Stm (ctx_cat Γ (alt__Δ K)) τ)
+        (P : forall (K : 𝑼𝑲 U), L) (Q : Lit τ -> LocalStore Γ -> L) :
+        (forall (K : 𝑼𝑲 U) (δΔ : LocalStore (alt__Δ K)),
+            env_cat δ δΔ ⊢ ⦃ P K ⦄ alt__r K ⦃ fun v δ' => Q v (env_drop (alt__Δ K) δ') ⦄) ->
+        δ ⊢
+          ⦃ ∀ (K : 𝑼𝑲 U) (v : Lit (𝑼𝑲_Ty K)), !!(eval e δ = 𝑼_fold (existT K v)) --> P K ⦄
+          stm_match_union U e (fun K => @alt Γ (𝑼𝑲_Ty K) τ (alt__Δ K) (alt__p K) (alt__r K))
+          ⦃ Q ⦄
+    | rule_stm_match_record
+        {R : 𝑹} {Δ : Ctx (𝑿 * Ty)} (e : Exp Γ (ty_record R))
+        (p : RecordPat (𝑹𝑭_Ty R) Δ) {τ : Ty} (rhs : Stm (ctx_cat Γ Δ) τ)
+        (P : L) (Q : Lit τ -> LocalStore Γ -> L) :
+        (forall (δΔ : LocalStore Δ),
+            env_cat δ δΔ ⊢ ⦃ P ⦄ rhs ⦃ fun v δ' => Q v (env_drop Δ δ') ⦄) ->
+        δ ⊢ ⦃ P ⦄ stm_match_record R e p rhs ⦃ Q ⦄
+    | rule_stm_read_register {σ : Ty} (r : 𝑹𝑬𝑮 σ) (v : Lit σ) :
+        δ ⊢ ⦃ r ↦ v ⦄ stm_read_register r ⦃ fun v' δ' => !!(δ' = δ) ∧ !!(v' = v) ∧ r ↦ v ⦄
+    (* | rule_stm_read_register_backwards {σ : Ty} (r : 𝑹𝑬𝑮 σ) *)
+    (*                                    (Q : Lit σ -> LocalStore Γ -> L) *)
+    (*                                    (v : Lit σ) : *)
+    (*     δ ⊢ ⦃ r ↦ v ✱ (r ↦ v -✱ Q v δ) ⦄ stm_read_register r ⦃ Q ⦄ *)
+    | rule_stm_write_register {σ : Ty} (r : 𝑹𝑬𝑮 σ) (w : Exp Γ σ)
+                              (Q : Lit σ -> LocalStore Γ -> L)
+                              (v : Lit σ) :
+        δ ⊢ ⦃ r ↦ v ⦄ stm_write_register r w ⦃ fun v' δ' => !!(δ' = δ) ∧ !!(v' = eval w δ)
+                                                         ∧ r ↦ v' ⦄
+    (* | rule_stm_write_register_backwards {σ : Ty} (r : 𝑹𝑬𝑮 σ) (w : Exp Γ σ) *)
+    (*                                     (Q : Lit σ -> LocalStore Γ -> L) *)
+    (*                                     (v : Lit σ) : *)
+    (*     δ ⊢ ⦃ r ↦ v ✱ (r ↦ eval w δ -✱ Q (eval w δ) δ) ⦄ stm_write_register r w ⦃ Q ⦄ *)
+    | rule_stm_assign_backwards
+        (x : 𝑿) (σ : Ty) (xIn : (x,σ) ∈ Γ) (s : Stm Γ σ)
+        (P : L) (R : Lit σ -> LocalStore Γ -> L) :
+        δ ⊢ ⦃ P ⦄ s ⦃ fun v δ' => R v (δ' ⟪ x ↦ v ⟫)%env ⦄ ->
+        δ ⊢ ⦃ P ⦄ stm_assign x s ⦃ R ⦄
+    | rule_stm_assign_forwards
+        (x : 𝑿) (σ : Ty) (xIn : (x,σ) ∈ Γ) (s : Stm Γ σ)
+        (P : L) (R : Lit σ -> LocalStore Γ -> L) :
+        δ ⊢ ⦃ P ⦄ s ⦃ R ⦄ ->
+        δ ⊢ ⦃ P ⦄ stm_assign x s ⦃ fun v__new δ' => ∃ v__old, R v__new (δ' ⟪ x ↦ v__old ⟫)%env ⦄
+    | rule_stm_call_forwards
+        {Δ σ} (f : 𝑭 Δ σ) (es : NamedEnv (Exp Γ) Δ)
+        (P : L)
+        (Q : Lit σ -> L) :
+        CTriple Δ (evals es δ) P Q (CEnv f) ->
+        δ ⊢ ⦃ P ⦄ stm_call f es ⦃ fun v δ' => Q v ∧ !!(δ = δ') ⦄
+    (* | rule_stm_call_backwards *)
+    (*     {Δ σ} (f : 𝑭 Δ σ) (es : NamedEnv (Exp Γ) Δ) *)
+    (*     (P : L) (Q : Lit σ -> LocalStore Γ -> L) : *)
+    (*     CTriple Δ (evals es δ) P (fun v => Q v δ) (CEnv f) -> *)
+    (*     δ ⊢ ⦃ P ⦄ stm_call f es ⦃ Q ⦄ *)
+    | rule_stm_call_frame
+        (Δ : Ctx (𝑿 * Ty)) (δΔ : LocalStore Δ) (τ : Ty) (s : Stm Δ τ)
+        (P : L) (Q : Lit τ -> LocalStore Γ -> L) :
+        δΔ ⊢ ⦃ P ⦄ s ⦃ fun v _ => Q v δ ⦄ ->
+        δ ⊢ ⦃ P ⦄ stm_call_frame Δ δΔ τ s ⦃ Q ⦄
+    | rule_stm_bind
+        {σ τ : Ty} (s : Stm Γ σ) (k : Lit σ -> Stm Γ τ)
+        (P : L) (Q : Lit σ -> LocalStore Γ -> L)
+        (R : Lit τ -> LocalStore Γ -> L) :
+        δ ⊢ ⦃ P ⦄ s ⦃ Q ⦄ ->
+        (forall (v__σ : Lit σ) (δ' : LocalStore Γ),
+            δ' ⊢ ⦃ Q v__σ δ' ⦄ k v__σ ⦃ R ⦄) ->
+        δ ⊢ ⦃ P ⦄ stm_bind s k ⦃ R ⦄
+    where "δ ⊢ ⦃ P ⦄ s ⦃ Q ⦄" := (@Triple _ δ _ P s Q).
+
+    Context {LLL : ILogicLaws L _}.
+    Lemma rule_consequence_right {Γ : Ctx (𝑿 * Ty)} {δ : LocalStore Γ} {σ : Ty}
+      {P : L} {Q Q' : Lit σ -> LocalStore Γ -> L} {s : Stm Γ σ} :
+      δ ⊢ ⦃ P ⦄ s ⦃ Q ⦄ -> (forall v δ, Q v δ ⊢ Q' v δ) -> δ ⊢ ⦃ P ⦄ s ⦃ Q' ⦄.
+    Proof.
+      intros H hyp. exact (rule_consequence δ (entails_refl P) hyp H).
+    Qed.
+
+  End Triples.
+
+  Notation "δ ⊢ ⦃ P ⦄ s ⦃ Q ⦄" := (@Triple _ _ _ δ _ P s Q).
 
 End ProgramLogic.
